Core/Metatheory/Determined/Semantic.lean
@@ -2,40 +2,82 @@ import LeanSubst
 import Core.Term
 import Core.Reduction
 import Core.Typing
-import Core.Metatheory.SpineType
+import Core.Metatheory.Determined.Definition
+import Core.Metatheory.GlobalWf
 
 open LeanSubst
 
 namespace Core
-def Term.Determined (t : Term) : Prop :=
-  VariantMissing [.ctor2 .choice, .ctor0 .zero, .guard] t
-
-def SpineElem.Determined : SpineElem -> Prop
-| type _ => True
-| term t => t.Determined
-| oterm t => t.Determined
-
-def Determined.openm (G : List Global) (x : String) : Prop := sorry
-  -- ∀ Δ Γ T sp,
-  --   lookup x G = some (.openm x T) ->
-  --   sp.length ≥ T.arity ->
-  --   SpineType g#x G Δ Γ sp T ->
-  --   ∃ t, Plus (Red G) ((g#x).apply sp) t ∧ Term.Determined t
-
-def Determined.defn (G : List Global) (x : String) : Prop :=
-  ∀ T t,
-    lookup x G = some (.defn x T t) ->
-    Term.Determined t
-
-def Global.Determined (G : List Global) : Prop :=
-  ∀ x, Determined.openm G x ∧ Determined.defn G x
 
 theorem determined_progress :
+  ⊢ G ->
   G&[],[] ⊢ t : A ->
   t.Determined ->
   Global.Determined G ->
   Value G t ∨ (∃ t', Plus (Red G) t t' ∧ t'.Determined)
 := by
-  sorry
+  intro wf j h1 h2
+  generalize Δdef : [] = Δ at j
+  generalize Γdef : [] = Γ at j
+  induction j
+  case var j1 j2 => subst Γdef; simp at j1
+  case global x A Δ b Γ j1 j2 =>
+    cases q1 : is_stable G x
+    case _ =>
+      have lem := not_stable_implies_openm_or_defn q1
+      rw [j1] at lem; simp at lem
+      cases lem
+      case _ q2 =>
+        apply Or.inr
+        obtain ⟨T, t, lem⟩ := Global.get_defn q2
+        replace h2 := (h2 x).2 T t lem
+        exists t; apply And.intro _ h2
+        apply Plus.start
+        have lem2 := @Red.defn G g#x x [] t (by simp [Term.spine])
+        simp at lem2; apply lem2
+        simp [lookup_defn]; rw [lem]; simp
+      case _ q2 =>
+        cases h : A.arity
+        case zero =>
+          obtain ⟨T, lem1⟩ := Global.get_openm q2
+          have lem2 := j1
+          simp [lookup_type] at j1; rw [lem1] at j1; simp [Entry.type] at j1
+          subst j1
+          apply Or.inr
+          replace h2 := (h2 x).1 Δ Γ T T [] lem1
+          simp [Term.apply] at h2
+          apply h2; apply Typing.global lem2 j2; apply h
+        case succ a =>
+          apply Or.inl; apply Value.app (x := x) (sp := [])
+          all_goals try simp [Term.spine]
+          apply Or.inr; simp [OpenVarVal]
+          apply And.intro q2; intro T q3
+          rw [j1] at q3; injection q3 with e; subst e
+          omega
+    case _ =>
+      apply Or.inl; apply Value.app (x := x) (sp := [])
+      all_goals try simp [Term.spine]
+      apply Or.inl q1
+  case mtch => sorry
+  case guard => sorry
+  case lam => sorry
+  case app Δ A b Γ f B a j1 j2 j3 ih1 ih2 =>
+    obtain ⟨df, da⟩ := Term.Determined.app.2 h1
+    replace ih1 := ih1 df Δdef Γdef
+    sorry
+  case lamt => sorry
+  case appt => sorry
+  case cast => sorry
+  case refl => sorry
+  case sym => sorry
+  case seq => sorry
+  case appc => sorry
+  case arrowc => sorry
+  case fst => sorry
+  case snd => sorry
+  case allc => sorry
+  case apptc => sorry
+  case zero => sorry
+  case choice => sorry
 
 end Core
