Core/Metatheory/Determined/Definition.lean
@@ -1,0 +1,72 @@
+import LeanSubst
+import Core.Term
+import Core.Reduction
+import Core.Typing
+
+open LeanSubst
+
+namespace Core
+
+def Term.Determined (t : Term) : Prop :=
+  VariantMissing [.ctor2 .choice, .ctor0 .zero, .guard] t
+
+def SpineElem.Determined : SpineElem -> Prop
+| type _ => True
+| term t => t.Determined
+| oterm t => t.Determined
+
+def Determined.openm (G : List Global) (x : String) : Prop :=
+  ∀ Δ Γ T B sp,
+    lookup x G = some (.openm x T) ->
+    G&Δ,Γ ⊢ (g#x).apply sp : B ->
+    sp.length ≥ T.arity ->
+    (∀ e ∈ sp, ∀ t, .oterm t = e -> t.spine.isSome) ->
+    (∀ e ∈ sp, ∀ t, .oterm t = e -> Value G t) ->
+    (∀ e ∈ sp, e.Determined) ->
+    ∃ t, Plus (Red G) ((g#x).apply sp) t ∧ Term.Determined t
+
+def Determined.defn (G : List Global) (x : String) : Prop :=
+  ∀ T t,
+    lookup x G = some (.defn x T t) ->
+    Term.Determined t
+
+def Global.Determined (G : List Global) : Prop :=
+  ∀ x, Determined.openm G x ∧ Determined.defn G x
+
+
+theorem Term.Determined.var : (#x).Determined := by
+  unfold Term.Determined; apply VariantMissing.var
+
+theorem Term.Determined.global : (g#x).Determined := by
+  unfold Term.Determined; apply VariantMissing.global
+
+theorem Term.Determined.lam : t.Determined -> (λ[A] t).Determined := by
+  intro h; unfold Term.Determined; apply VariantMissing.lam; apply h
+
+theorem Term.Determined.lamt : t.Determined -> (Λ[A] t).Determined := by
+  intro h; unfold Term.Determined; apply VariantMissing.tbind _ h;
+  intro h';
+  cases h'; case _ h => cases h; case _ h => cases h; case _ h => cases h
+
+theorem Term.Determined.app {f a : Term} : f.Determined ∧ a.Determined <-> (f •(b) a).Determined := by
+  apply Iff.intro <;> intro h
+  unfold Term.Determined; apply VariantMissing.ctor2 _ h.1 h.2
+  intro h'; cases h'; case _ h => cases h; case _ h => cases h; case _ h => cases h
+  cases h; unfold Determined; simp [*]
+
+theorem Term.Determined.appt {f: Term} {a : Ty} : f.Determined -> (f •[ a ]).Determined := by
+  intro h1
+  unfold Term.Determined; apply VariantMissing.ctor1 _ h1
+  intro h'; cases h'; case _ h => cases h; case _ h => cases h; case _ h => cases h
+
+theorem Term.Determined.match {s d : Term} {ps cs : Vect n Term}:
+  s.Determined ->
+  d.Determined ->
+  (∀ i, (ps i).Determined) ->
+  (∀ i, (cs i).Determined) ->
+  (match! n s ps cs d).Determined
+:= by
+  intro h1 h2 h3 h4
+  unfold Term.Determined; apply VariantMissing.mtch; repeat assumption
+
+end Core
